Stlc/context.lean
@@ -1,73 +1,74 @@
 import Stlc.basics
-import Mathlib.Data.Finset.Basic
-import Mathlib.Data.List.Basic
 
 /-
-In order to make typing judgments, we need the notion of context. 
+In order to make typing judgments, we need the notion of context.
 The definition is designed to talk about "(x : T)"-like assumptions.
 -/
-open List 
+open List
 
 notation "context" => List (ℕ × Typ)
 
 @[simp]
-def dom : context → (Finset ℕ)
-| [] => ∅ 
-| ((x, _) :: Γ') => {x} ∪ (dom Γ') 
+def context_terms : context → (Finset ℕ)
+| [] => ∅
+| ((x, _) :: Γ') => {x} ∪ (context_terms Γ')
 
 @[simp]
-def in_list (a : ℕ) : context → Prop 
+def in_context (a : ℕ) : context → Prop
 | [] => False
-| (b :: m) => (a = b.1) ∨ (in_list a m)
+| (b :: m) => (a = b.1) ∨ (in_context a m)
 
-lemma dom_iff_in_list (a : ℕ) (Γ : context) : (a ∈ dom Γ) ↔ in_list a Γ := by
+lemma context_terms_iff_in_list (a : ℕ) (Γ : context) :
+    (a ∈ context_terms Γ) ↔ in_context a Γ := by
   induction Γ
   case nil =>
-    simp only [dom, Finset.not_mem_empty, in_list]
+    simp only [context_terms, Finset.not_mem_empty, in_context]
   case cons b Γ' f =>
-    simp only [dom, Finset.mem_union, Finset.mem_singleton, in_list]
-    rw [f]  
+    simp only [context_terms, Finset.mem_union, Finset.mem_singleton, in_context]
+    rw [f]
 
-lemma in_list_cons_neg (a : ℕ) (Γ Δ : context) :
-    ¬ (in_list a (Γ ++ Δ)) → ¬ (in_list a Γ) ∧ ¬ (in_list a Δ) := by
+lemma in_context_append_neg (a : ℕ) (Γ Δ : context) :
+    ¬ (in_context a (Γ ++ Δ)) → ¬ (in_context a Γ) ∧ ¬ (in_context a Δ) := by
   intro H
   induction Γ
   case nil =>
-    simp only [in_list, not_false_eq_true, true_and] at H ⊢
+    simp only [in_context, not_false_eq_true, true_and] at H ⊢
     rwa [nil_append] at H
   case cons b Γ' f =>
-    simp only [in_list] at H f ⊢
+    simp only [in_context] at H f ⊢
     push_neg at H ⊢
-    exact ⟨⟨H.1, (f (H.2)).1⟩, (f (H.2)).2⟩   
+    exact ⟨⟨H.1, (f (H.2)).1⟩, (f (H.2)).2⟩
 
-lemma in_list_cons_neg' (a : ℕ) (Γ Δ : context) :
-    ¬ (in_list a Γ) ∧ ¬ (in_list a Δ) → ¬ (in_list a (Γ ++ Δ)) := by
+lemma in_context_append_neg' (a : ℕ) (Γ Δ : context) :
+    ¬ (in_context a Γ) ∧ ¬ (in_context a Δ) → ¬ (in_context a (Γ ++ Δ)) := by
   rintro ⟨H1, H2⟩
   induction Γ
   case nil =>
     simp only [nil_append]
     exact H2
   case cons b Γ' f =>
-    simp only [in_list, append_eq] at H1 ⊢
-    push_neg at H1 ⊢ 
-    exact ⟨H1.1, f H1.2⟩ 
+    simp only [in_context, append_eq] at H1 ⊢
+    push_neg at H1 ⊢
+    exact ⟨H1.1, f H1.2⟩
 
 -- We can only bind variable once per context --
-inductive valid_ctx : context → Prop where 
+inductive valid_ctx : context → Prop where
 | valid_nil : valid_ctx []
-| valid_cons (Γ : context) (x : ℕ) (T : Typ) : (valid_ctx Γ) → (¬ (in_list x Γ)) → valid_ctx ((x, T) :: Γ)
+| valid_cons (Γ : context) (x : ℕ) (T : Typ) :
+    (valid_ctx Γ) → (¬ (in_context x Γ)) → valid_ctx ((x, T) :: Γ)
 
 open valid_ctx
 
 --Properties of valid contexts
 lemma valid_push (Γ : context) (x : ℕ) (T : Typ) :
-      valid_ctx Γ → ¬ (in_list x Γ) → valid_ctx ([(x, T)] ++ Γ) := by
+    valid_ctx Γ → ¬ (in_context x Γ) → valid_ctx ([(x, T)] ++ Γ) := by
   simp only [singleton_append]
   exact (valid_cons Γ x T)
 
-lemma valid_remove_mid (Γ Δ Ψ : context) : valid_ctx (Ψ ++ Δ ++ Γ) -> valid_ctx (Ψ ++ Γ) := by
+lemma valid_remove_mid (Γ Δ Ψ : context) :
+    valid_ctx (Ψ ++ Δ ++ Γ) -> valid_ctx (Ψ ++ Γ) := by
   induction Ψ
-  case nil => 
+  case nil =>
     induction Δ
     case nil =>
       simp only [append_nil, nil_append, imp_self]
@@ -82,26 +83,26 @@ lemma valid_remove_mid (Γ Δ Ψ : context) : valid_ctx (Ψ ++ Δ ++ Γ) -> vali
     intro H
     cases H
     next x S p p' =>
-      simp only [cons_append, append_assoc] at f p ⊢ 
+      simp only [cons_append, append_assoc] at f p ⊢
       apply valid_cons
       exact (f p)
-      apply in_list_cons_neg'
+      apply in_context_append_neg'
       constructor
-      exact (in_list_cons_neg _ _ _ p').1
-      exact (in_list_cons_neg _ _ _ (in_list_cons_neg _ _ _ p').2).2
+      exact (in_context_append_neg _ _ _ p').1
+      exact (in_context_append_neg _ _ _ (in_context_append_neg _ _ _ p').2).2
 
 lemma valid_remove_mid_cons (x : ℕ) (T : Typ) (Γ Δ : context) :
-    valid_ctx (Δ ++ (x, T) :: Γ) → 
-    valid_ctx (Δ ++ Γ) := by
+    valid_ctx (Δ ++ (x, T) :: Γ)
+    → valid_ctx (Δ ++ Γ) := by
   intro H
   simp only [append_cons Δ (x, T) Γ] at H
   apply valid_remove_mid
   exact H
 
 lemma valid_remove_cons (x : ℕ) (T : Typ) (Γ : context) :
-    valid_ctx ((x, T) :: Γ) → 
-    valid_ctx (Γ) := by
-  intro H 
+    valid_ctx ((x, T) :: Γ)
+    → valid_ctx (Γ) := by
+  intro H
   rw [← nil_append Γ]
   apply valid_remove_mid_cons
   simp
@@ -122,15 +123,19 @@ lemma binds_singleton (x : ℕ) (T : Typ) : binds x T [(x, T)] := by
   simp only [_root_.get]
   simp only [ite_true]
 
-lemma binds_tail (x : ℕ) (T : Typ) (Γ Δ : context) : 
-    binds x T Γ → (¬ (in_list x Δ)) → binds x T (Δ ++ Γ) := by
+lemma binds_singleton_tail (x : ℕ) (T : Typ) (Γ : context) :
+    binds x T ([(x, T)] ++ Γ) := by
+  simp only [binds, _root_.get, append_eq, nil_append, ite_true]
+
+lemma binds_tail (x : ℕ) (T : Typ) (Γ Δ : context) :
+    binds x T Γ → (¬ (in_context x Δ)) → binds x T (Δ ++ Γ) := by
   intro bx nx
   simp [binds] at bx ⊢
   induction Δ
   case nil =>
     simp only [nil_append, bx]
   case cons b Δ' f' =>
-    simp [in_list] at nx
+    simp [in_context] at nx
     push_neg at nx
     simp only [_root_.get, append_eq]
     rw [if_neg nx.1]
@@ -155,10 +160,12 @@ lemma binds_head (x : ℕ) (T : Typ) (Γ Δ : context) :
 
 --Case analysis on binds
 lemma binds_concat_inv' (x : ℕ) (T : Typ) (Γ Δ : context) :
-    binds x T (Γ ++ Δ) → ((in_list x Γ) ∨ ¬(binds x T Δ)) → (binds x T Γ) := by 
+    binds x T (Γ ++ Δ)
+    → ((in_context x Γ) ∨ ¬(binds x T Δ))
+    → (binds x T Γ) := by
   induction Γ
   case nil =>
-    simp only [binds, nil_append, _root_.get, in_list]
+    simp only [binds, nil_append, _root_.get, in_context]
     simp only [false_or]
     exact (fun p f => f p)
   case cons b Γ' f =>
@@ -170,7 +177,7 @@ lemma binds_concat_inv' (x : ℕ) (T : Typ) (Γ Δ : context) :
       . simp [if_neg hxb] at bxT ⊢
         apply f
         exact bxT
-        simp [in_list, hxb] at h1
+        simp [in_context, hxb] at h1
         left
         exact h1
     . simp only [binds, _root_.get]
@@ -184,7 +191,8 @@ lemma binds_concat_inv' (x : ℕ) (T : Typ) (Γ Δ : context) :
         exact h2
 
 lemma binds_concat_inv (x : ℕ) (T : Typ) (Γ Δ : context) :
-    binds x T (Γ ++ Δ) → ((¬ (in_list x Γ)) ∧ (binds x T Δ)) ∨ (binds x T Γ) := by 
+    binds x T (Γ ++ Δ)
+    → ((¬ (in_context x Γ)) ∧ (binds x T Δ)) ∨ (binds x T Γ) := by
   intro bxT
   refine Iff.mpr or_iff_not_imp_left ?_
   intro H
@@ -192,7 +200,8 @@ lemma binds_concat_inv (x : ℕ) (T : Typ) (Γ Δ : context) :
   push_neg at H
   exact Iff.mpr or_iff_not_imp_left H
 
-lemma binds_singleton_inv (x y : ℕ) (X Y : Typ) : binds x X [(y,Y)] → (x = y) ∧ (X = Y) := by 
+lemma binds_singleton_inv (x y : ℕ) (X Y : Typ) :
+    binds x X [(y,Y)] → (x = y) ∧ (X = Y) := by
   simp only [binds, _root_.get]
   intro H
   by_cases hxy : x = y
@@ -201,7 +210,8 @@ lemma binds_singleton_inv (x y : ℕ) (X Y : Typ) : binds x X [(y,Y)] → (x = y
   . simp [if_neg hxy] at H
 
 lemma binds_mid (x : ℕ) (T : Typ) (Δ Γ : context) :
-    valid_ctx (Γ ++ [(x,T)] ++ Δ) -> binds x T (Γ ++ [(x,T)] ++ Δ) := by
+    valid_ctx (Γ ++ [(x,T)] ++ Δ)
+    → binds x T (Γ ++ [(x,T)] ++ Δ) := by
   induction Γ
   case nil =>
     simp only [nil_append, singleton_append, binds, _root_.get, append_eq, ite_true, implies_true]
@@ -212,16 +222,17 @@ lemma binds_mid (x : ℕ) (T : Typ) (Δ Γ : context) :
       simp only [binds, _root_.get, append_eq, append_assoc, singleton_append] at f H' g ⊢
       by_cases hxy : x = y
       . simp [if_pos hxy]
-        have ⟨_, t2⟩ := in_list_cons_neg _ _ _ g
+        have ⟨_, t2⟩ := in_context_append_neg _ _ _ g
         simp at t2
         push_neg at t2
         by_contra _
         exact (t2.1 hxy.symm)
       . simp [if_neg hxy]
-        exact (f H') 
+        exact (f H')
 
 lemma binds_mid_eq (x : ℕ) (T S : Typ) (Γ Δ : context) :
-    binds x T (Δ ++ [(x,S)] ++ Γ) → valid_ctx (Δ ++ [(x,S)] ++ Γ) →  T = S := by
+    binds x T (Δ ++ [(x,S)] ++ Γ)
+    → valid_ctx (Δ ++ [(x,S)] ++ Γ) →  T = S := by
   induction Δ
   case nil =>
     simp only [binds, _root_.get, append_eq, nil_append, ite_true, Option.some.injEq, singleton_append]
@@ -232,27 +243,29 @@ lemma binds_mid_eq (x : ℕ) (T S : Typ) (Γ Δ : context) :
     next y S' H' g =>
       simp only [binds, _root_.get, append_eq, append_assoc, singleton_append] at p f H' g ⊢
       by_cases hxy : x = y
-      . have ⟨_, t2⟩ := in_list_cons_neg _ _ _ g
+      . have ⟨_, t2⟩ := in_context_append_neg _ _ _ g
         simp at t2
         push_neg at t2
         by_contra _
         exact (t2.1 hxy.symm)
-      . simp [if_neg hxy] at p 
+      . simp [if_neg hxy] at p
         exact (f p H')
-        
+
 lemma binds_mid_eq_cons (x : ℕ) (T S : Typ) (Γ Δ : context) :
-    binds x T (Δ ++ (x,S) :: Γ) → valid_ctx (Δ ++ (x,S) :: Γ) → T = S := by
+    binds x T (Δ ++ (x,S) :: Γ)
+    → valid_ctx (Δ ++ (x,S) :: Γ) → T = S := by
   intro p H
   simp only [append_cons Δ (x, S) Γ] at p H
   exact (binds_mid_eq x T S Γ Δ p H)
 
 --Additional properties of binds
-lemma binds_in (x : ℕ) (T : Typ) (Γ : context) : binds x T Γ → in_list x Γ := by
+lemma binds_in_context (x : ℕ) (T : Typ) (Γ : context) :
+    binds x T Γ → in_context x Γ := by
   induction Γ
   case nil =>
-    simp only [binds, _root_.get, in_list, IsEmpty.forall_iff]
+    simp only [binds, _root_.get, in_context, IsEmpty.forall_iff]
   case cons b Γ' f =>
-    simp only [binds, _root_.get, in_list] at f ⊢ 
+    simp only [binds, _root_.get, in_context] at f ⊢
     by_cases hxb : x = b.1
     . simp only [if_pos hxb]
       intro _
@@ -261,36 +274,37 @@ lemma binds_in (x : ℕ) (T : Typ) (Γ : context) : binds x T Γ → in_list x �
       intro p
       exact (Or.inr (f p))
 
-lemma binds_fresh (x : ℕ) (T : Typ) (Γ : context) : ¬ in_list x Γ → ¬ binds x T Γ := by
+lemma binds_fresh (x : ℕ) (T : Typ) (Γ : context) :
+    ¬ in_context x Γ → ¬ binds x T Γ := by
   contrapose
   simp only [not_not]
-  exact (binds_in x T Γ)
+  exact (binds_in_context x T Γ)
 
 lemma binds_concat_ok (x : ℕ) (T : Typ) (Γ Δ : context) :
     binds x T Γ -> valid_ctx (Δ ++ Γ) -> binds x T (Δ ++ Γ) := by
   induction Δ
-  case nil => 
+  case nil =>
     simp only [binds, nil_append]
     exact (fun p _ => p)
   case cons b Δ' f =>
     intro p H
     cases H
     next y S H' g =>
-      simp only [binds, _root_.get, append_eq] at H' ⊢ 
+      simp only [binds, _root_.get, append_eq] at H' ⊢
       by_cases hxy : x = y
       . simp only [if_pos hxy]
         by_contra
         apply g
-        apply binds_in y T (Δ' ++ Γ)
+        apply binds_in_context y T (Δ' ++ Γ)
         rw [← hxy]
         exact (f p H')
       . simp only [if_neg hxy]
         exact (f p H')
 
 lemma binds_weaken (x : ℕ) (T : Typ) (Γ Δ Ψ: context) :
-    binds x T (Ψ ++ Γ) ->
-    valid_ctx (Ψ ++ Δ ++ Γ) ->
-    binds x T (Ψ ++ Δ ++ Γ) := by
+    binds x T (Ψ ++ Γ)
+    → valid_ctx (Ψ ++ Δ ++ Γ)
+    → binds x T (Ψ ++ Δ ++ Γ) := by
   induction Ψ
   case nil =>
     simp only [binds, nil_append]
@@ -299,22 +313,20 @@ lemma binds_weaken (x : ℕ) (T : Typ) (Γ Δ Ψ: context) :
     intro p H
     cases H
     next y S H' g =>
-      simp only [binds, _root_.get, append_eq, append_assoc, in_list] at f H' p g ⊢ 
+      simp only [binds, _root_.get, append_eq, append_assoc, in_context] at f H' p g ⊢
       by_cases hxy : x = y
-      . simp only [if_pos hxy] at p ⊢ 
+      . simp only [if_pos hxy] at p ⊢
         exact p
-      . simp only [if_neg hxy] at p ⊢ 
+      . simp only [if_neg hxy] at p ⊢
         exact (f p H')
-        
+
 lemma binds_weaken_at_head (x : ℕ) (T : Typ) (Γ Δ : context) :
-    binds x T Δ → 
-    valid_ctx (Γ ++ Δ) → 
-    binds x T (Γ ++ Δ) := (binds_weaken x T Δ Γ [])
+    binds x T Δ → valid_ctx (Γ ++ Δ)
+    → binds x T (Γ ++ Δ) := (binds_weaken x T Δ Γ [])
 
 lemma binds_remove_mid (x y : ℕ) (T S : Typ) (Γ Δ : context) :
-    binds x T (Γ ++ ([(y,S)] ++ Δ)) → 
-    x ≠ y → 
-    binds x T (Γ ++ Δ) := by
+    binds x T (Γ ++ ([(y,S)] ++ Δ))
+    → x ≠ y → binds x T (Γ ++ Δ) := by
   intro p H
   have t := (binds_concat_inv x T Γ ([(y,S)] ++ Δ) p)
   rcases t with ⟨t11, t12⟩ | t2
@@ -325,10 +337,9 @@ lemma binds_remove_mid (x y : ℕ) (T S : Typ) (Γ Δ : context) :
   . apply (binds_head _ _ _ _ t2)
 
 lemma binds_remove_mid_cons  (x y : ℕ) (T S : Typ) (Γ Δ : context) :
-    binds x T (Δ ++ (y, S) :: Γ) → 
-    x ≠ y → 
-    binds x T (Δ ++ Γ) := by
+    binds x T (Δ ++ (y, S) :: Γ)
+    → x ≠ y → binds x T (Δ ++ Γ) := by
   intro H p
   apply (binds_remove_mid x y T S Δ Γ)
   rwa [append_cons, append_assoc] at H
-  exact p 
+  exact p
