Stlc/confluence.lean
@@ -3,8 +3,6 @@ import Stlc.open_close
 import Stlc.context
 import Stlc.typing
 import Stlc.reductions
-import Mathlib.Data.Finset.Basic
-import Mathlib.Data.List.Basic
 
 open Typ
 open Trm
@@ -17,8 +15,8 @@ open multi_red
 open multi_para
 
 lemma para_diamond t t1 :
-    para t t1 → ∀ t2, para t t2 →
-    ∃ t', (para t1 t') ∧ (para t2 t') := by
+    para t t1 → ∀ t2, para t t2
+    → ∃ t', (para t1 t') ∧ (para t2 t') := by
   intro tpt1
   induction tpt1
   case para_var x =>
@@ -29,8 +27,7 @@ lemma para_diamond t t1 :
     intro t2 tpt2
     cases tpt2
     case para_red u1' u2' L' f' s2pu2' =>
-      have q := pick_fresh u2' (L ∪ L' ∪ (fv u1') ∪ (fv s1') ∪ (fv s2'))
-      rcases q with ⟨x, qx⟩
+      let ⟨x, qx⟩ := pick_fresh u2' (L ∪ L' ∪ (fv u1') ∪ (fv s1') ∪ (fv s2'))
       simp at qx
       push_neg at qx
       rw [subst_intro u1' u2' (para_regular _ _ s2pu2').2 x qx.2.2.1]
@@ -48,8 +45,7 @@ lemma para_diamond t t1 :
     case para_app u2 u2' s1pu2 s2pu2' =>
       cases s1pu2
       next s1'' L' f' =>
-        have q := pick_fresh s1' (L ∪ L' ∪ (fv s1''))
-        rcases q with ⟨x, qx⟩
+        let ⟨x, qx⟩ := pick_fresh s1' (L ∪ L' ∪ (fv s1''))
         simp at qx
         push_neg at qx
         have fact1: ∃ t', para s2' t' ∧ para u2' t' := by
@@ -68,15 +64,14 @@ lemma para_diamond t t1 :
           intro y qy
           rw [← close_open_var x s1'' qx.2.2.1]
           apply open_close_para _ _ _ _ qt''.2 qy
-          exact qt'.2        
+          exact qt'.2
   case para_app s1 s1' s2 s2' s1ps1' _ ih1 ih2 =>
       intro t2 tpt2
       cases tpt2
       case para_red t1' u1' u2' L f s2pu2' =>
         cases s1ps1'
         next s1'' L' f' =>
-          have q := pick_fresh u1' (L ∪ L' ∪ (fv s1''))
-          rcases q with ⟨x, qx⟩
+          let ⟨x, qx⟩ := pick_fresh u1' (L ∪ L' ∪ (fv s1''))
           simp at qx
           push_neg at qx
           have fact1: ∃ t', para s2' t' ∧ para u2' t' := by
@@ -108,28 +103,28 @@ lemma para_diamond t t1 :
     intro t2 tpt2
     cases tpt2
     next t2' L' f' =>
-      have q := pick_fresh s2' (L ∪ L' ∪ (fv t2'))
-      rcases q with ⟨x, qx⟩
+      let ⟨x, qx⟩ := pick_fresh s2' (L ∪ L' ∪ (fv t2'))
       simp at qx
       push_neg at qx
       have fact1 := ih x qx.1 _ (f' x qx.2.1)
       rcases fact1 with ⟨t', qt'⟩
       use (λ (close₀ t' x))
       constructor
-      . apply para_abs _ _ (fv (open₀ s2' ($ x)) ∪ fv t' ∪ {x}) 
+      . apply para_abs _ _ (fv (open₀ s2' ($ x)) ∪ fv t' ∪ {x})
         intro y qy
         rw [← close_open_var x s2' qx.2.2.2]
         apply open_close_para _ _ _ _ qt'.1 qy
-      . apply para_abs _ _ (fv (open₀ t2' ($ x)) ∪ fv t' ∪ {x}) 
+      . apply para_abs _ _ (fv (open₀ t2' ($ x)) ∪ fv t' ∪ {x})
         intro y qy
         rw [← close_open_var x t2' qx.2.2.1]
         apply open_close_para _ _ _ _ qt'.2 qy
 
-  
-lemma multi_para_diamond_core t t1 t2 : (para t t1) ∧ (multi_para t t2) → ∃ t', (multi_para t1 t') ∧ (para t2 t') := by
+lemma multi_para_diamond_core t t1 t2 :
+    (para t t1) ∧ (multi_para t t2)
+    → ∃ t', (multi_para t1 t') ∧ (para t2 t') := by
   intro ⟨tpt1, tmt2⟩
   induction tmt2
-  case m_para_refl _ => 
+  case m_para_refl _ =>
     use t1
     constructor
     apply m_para_refl
@@ -142,10 +137,11 @@ lemma multi_para_diamond_core t t1 t2 : (para t t1) ∧ (multi_para t t2) → �
     use t''
     constructor
     exact (m_para_head _ _ _ h1 h4)
-    exact h3  
+    exact h3
 
-
-lemma multi_para_diamond t t1 t2 : (multi_para t t1) ∧ (multi_para t t2) → ∃ t', (multi_para t1 t') ∧ (multi_para t2 t') := by
+lemma multi_para_diamond t t1 t2 :
+    (multi_para t t1) ∧ (multi_para t t2)
+    → ∃ t', (multi_para t1 t') ∧ (multi_para t2 t') := by
   intro ⟨tmpt1 , tmpt2⟩
   induction tmpt1
   case m_para_refl _ =>
@@ -154,15 +150,15 @@ lemma multi_para_diamond t t1 t2 : (multi_para t t1) ∧ (multi_para t t2) → �
   case m_para_head s1 s2 _ s1ps2 f =>
     rcases f with ⟨t', ⟨h1,h2⟩⟩
     have q := (multi_para_diamond_core _ _ _ ⟨s1ps2, h1⟩)
-    rcases q with ⟨t'', ⟨h3, h4⟩⟩ 
+    rcases q with ⟨t'', ⟨h3, h4⟩⟩
     use t''
     constructor
     exact h3
     exact (m_para_head _ _ _ h2 h4)
 
-theorem beta_red_confluence : 
-    ∀ t t1 t2, (multi_red t t1) ∧ (multi_red t t2) → 
-    ∃ t', (multi_red t1 t') ∧ (multi_red t2 t') := by
+theorem beta_red_confluence :
+    ∀ t t1 t2, (multi_red t t1) ∧ (multi_red t t2)
+    → ∃ t', (multi_red t1 t') ∧ (multi_red t2 t') := by
   intro t t1 t2 ⟨trt1 , trt2⟩
   simp [multi_red_iff_multi_para] at trt1 trt2 ⊢
   exact (multi_para_diamond t t1 t2 ⟨trt1 , trt2⟩)
