Stlc/multi_subst.lean
@@ -1,0 +1,211 @@
+import Stlc.basics
+import Stlc.context
+import Stlc.typing
+import Stlc.reductions
+import Stlc.confluence
+
+open Typ
+open Trm
+open subst
+open beta_red
+open multi_red
+open lc
+open typing
+
+namespace Trm
+
+-- Defining substitutions over contexts --
+@[simp]
+def multi_subst (L : Finset ℕ) (f : L → Trm) : Trm → Trm
+| bvar i => bvar i
+| fvar y => if h : (y ∈ L) then (f ⟨y, h⟩) else (fvar y)
+| abs u => abs (multi_subst L f u)
+| app u1 u2 => app (multi_subst L f u1) (multi_subst L f u2)
+
+-- context_type takes a term in a context and outputs its type
+@[simp]
+def context_type Γ (x : context_terms Γ) : Typ :=
+  match Γ, x with
+  | [], ⟨_, h⟩ => by simp [context_terms] at h
+  | (x, b) :: Γ, ⟨x', h⟩ =>
+    if ha : x' = x then
+      b
+    else
+      context_type Γ ⟨x', by simpa [context_terms, ha] using h⟩
+
+-- substitution over the empty context does nothing
+lemma multi_subst_over_empty_context t (f : context_terms [] → Trm) :
+    (multi_subst (context_terms []) f t) = t := by
+  induction t
+  case bvar i =>
+    simp
+  case fvar i =>
+    simp
+  case abs t' ih =>
+    simp at ih ⊢
+    rw [ih]
+  case app t1 t2 ih1 ih2 =>
+    simp at ih1 ih2 ⊢
+    exact ⟨ih1, ih2⟩
+
+-- substitution over [(x,T)] is the same as usual (single) substitution
+lemma multi_subst_at_singleton t x T :
+    (f : context_terms [(x, T)] → Trm)
+    → (multi_subst (context_terms [(x, T)]) f t)
+      = ([x // (f ⟨x, by simp⟩)] t) := by
+  intro f
+  induction t
+  case bvar i =>
+    simp
+  case fvar i =>
+    simp
+    by_cases h : i = x
+    . simp [h]
+    . simp [h]
+  case abs t' ih =>
+    simp
+    exact ih
+  case app t1 t2 ih1 ih2 =>
+    simp
+    exact ⟨ih1, ih2⟩
+
+-- if we have a function of terms of a context, say f,
+--for a term u and variable x, we can extend the f with mapping x → u
+@[simp]
+def add_term Γ (f : context_terms Γ → Trm)
+    (u : Trm) y T (x : context_terms ((y , T) :: Γ)) : Trm := by
+  rcases x with ⟨x' , h⟩
+  by_cases p : x' = y
+  . exact u
+  . simp [p] at h
+    exact f ⟨x' , h⟩
+
+--If y does not appear in t, then substitution over a context (y,T) ++ Γ
+--is the same as substitution over Γ
+lemma multi_subst_fresh Γ t u y T (h : y ∉ (fv t)) (f : context_terms Γ → Trm) :
+    (multi_subst (context_terms ((y , T) :: Γ)) (add_term Γ f u y T) t)
+     = (multi_subst (context_terms Γ) f t) := by
+  induction t
+  case bvar i =>
+    rfl
+  case fvar i =>
+    simp [fv] at h
+    simp only [multi_subst, context_terms, Finset.mem_union, Finset.mem_singleton, add_term]
+    have p : i ≠ y := fun q => h q.symm
+    simp [p]
+  case abs u hu =>
+    simp only [multi_subst, abs.injEq]
+    exact (hu h)
+  case app u1 u2 h1 h2 =>
+    simp only [multi_subst, app.injEq]
+    simp [fv] at h
+    push_neg at h
+    exact ⟨(h1 h.1), (h2 h.2)⟩
+
+
+--substitution over a context distributes over opening
+lemma multi_subst_open_lemma_1 e1 e2 Γ : (f : context_terms Γ → Trm)
+   → (∀ x (h : x ∈ context_terms Γ), lc (f ⟨x,h⟩)) → (j : ℕ)
+   → (multi_subst (context_terms Γ) f ({j ~> e2} e1))
+     = ({j ~> multi_subst (context_terms Γ) f e2} (multi_subst (context_terms Γ) f e1)) := by
+  induction e1
+  case bvar y =>
+    simp
+    intros f _ j
+    by_cases hjy : (j = y)
+    . simp [opening]
+      rw [if_pos, if_pos] <;> exact hjy
+    . simp [opening]
+      rw [if_neg, if_neg, multi_subst]
+      <;> exact hjy
+  case fvar y =>
+   intro f lcf j
+   by_cases hy : (y ∈ context_terms Γ)
+   . simp [opening, multi_subst, hy]
+     exact (opening_lc (f ⟨y, hy⟩) _ (lcf y hy) _)
+   . simp [opening, multi_subst, hy]
+  case abs u ihu =>
+   intro f lcf j
+   simp [opening, multi_subst]
+   exact (ihu f lcf (j + 1))
+  case app u1 u2 ihu1 ihu2 =>
+   intro f lcf j
+   simp [opening, multi_subst]
+   exact ⟨ihu1 f lcf j, ihu2 f lcf j⟩
+
+-- special case of previous fact at j=0
+lemma multi_subst_open_lemma_2 Γ t u y T : lc u → y ∉ fv t
+    → (f : context_terms Γ → Trm)
+    → (∀ x (h : x ∈ context_terms Γ), lc (f ⟨x,h⟩))
+    → (multi_subst (context_terms ((y , T) :: Γ)) (add_term Γ f u y T) (open₀ t ($ y)))
+      = (open₀ (multi_subst (context_terms Γ) f t) u) := by
+  intro lcu hy f lcf
+  rw [open₀ , multi_subst_open_lemma_1, multi_subst, ← open₀]
+  rw [multi_subst_fresh Γ t u y T hy f]
+  simp
+  intro x h
+  by_cases p : x = y
+  . simp [p]
+    exact lcu
+  . simp [p] at h ⊢
+    exact lcf x h
+
+--When we open a term, we can instead open the term with a fresh variable and
+--then multi-substitute for that variable.
+lemma multi_subst_open Γ t y : y ∉ context_terms Γ
+    → (f : context_terms Γ → Trm)
+    → (∀ x (h : x ∈ context_terms Γ), lc (f ⟨x,h⟩))
+    → (multi_subst (context_terms Γ) f (open₀ t ($ y)))
+      = (open₀ (multi_subst (context_terms Γ) f t) ($ y)) := by
+  intro hy f lcf
+  rw [open₀ , multi_subst_open_lemma_1, multi_subst, ← open₀]
+  simp [hy]
+  apply lcf
+
+--if (x,T) appears in context Γ, then the context map sends Γ x to T
+lemma context_type_eq_bind Γ (x : context_terms Γ) T :
+    valid_ctx Γ → binds x T Γ → context_type Γ x = T := by
+  induction Γ
+  case nil =>
+    intro _ bnd
+    cases bnd
+  case cons h Γ' ih =>
+    intro vld bnd
+    simp only [context_type, context_terms]
+    by_cases p : h.1 = ↑x
+    . simp [p] at bnd ⊢
+      apply bnd
+    . have q : (↑x ≠ h.1) := (fun z => p (z.symm))
+      simp [q]
+      apply ih
+      apply valid_remove_cons _ _ _ vld
+      apply binds_remove_mid_cons ↑x h.1 T h.2 Γ' [] bnd
+      symm
+      exact p
+
+-- if a term is locally closed, and there is list of locally closed terms, then
+-- substition with these terms is also locally closed.
+lemma multi_subst_lc t Γ : lc t
+    → (f : context_terms Γ → Trm)
+    → (∀ x (h : x ∈ context_terms Γ), lc (f ⟨x,h⟩))
+    → lc ((multi_subst (context_terms Γ) f t)) := by
+  intro lct f lcf
+  induction lct
+  case lc_var y =>
+    rw [multi_subst]
+    by_cases hxy : y ∈ context_terms Γ
+    . simp [if_pos, hxy]
+      exact (lcf y hxy)
+    . simp [if_neg, hxy]
+      exact (lc_var y)
+  case lc_abs u L a hu =>
+    simp
+    apply lc_abs _ (L ∪ (context_terms Γ) ∪ (fv u))
+    intro x hx
+    simp at hx
+    push_neg at hx
+    rw [← multi_subst_open Γ u x hx.2.1 f lcf]
+    apply hu x hx.1
+  case lc_app u1 u2 lcu1 lcu2 hu1 hu2 =>
+    dsimp [multi_subst]
+    apply (lc_app _ _ hu1 hu2)
