Stlc/normalization.lean
@@ -1,0 +1,385 @@
+import Stlc.basics
+import Stlc.context
+import Stlc.typing
+import Stlc.reductions
+import Stlc.confluence
+import Stlc.multi_subst
+
+open Typ
+open Trm
+open lc
+open typing
+
+namespace Trm
+
+--a term is reducible if it reducts
+def reducible (t : Trm) : Prop := ∃ t', beta_red t t'
+
+--a term is normal if it is not reducible
+def normal (t : Trm) : Prop := ¬ (reducible t)
+
+--a term is normal iff it has no multi-step reduct
+lemma normal_has_no_proper_multi_red (t : Trm) :
+    normal t → ∀ t', multi_red t t' → t = t' := by
+  intro nt t' tmt'
+  induction tmt'
+  case mr_refl _ =>
+    rfl
+  case mr_head t2 t3 tmt2 t2bt3 ih =>
+    by_contra p
+    rw [ih] at nt
+    apply nt
+    exact ⟨t3, t2bt3⟩
+
+-- a term is normalizable if it has a normal multi-step reduct
+def normalizable (t : Trm) : Prop := ∃ t', ((multi_red t t') ∧ (normal t'))
+
+-- a term t is strongly normalizable of any one-step reduction sequence
+--starting with t must terminate
+def strongly_normalizable (t : Trm) : Prop :=
+  ∀ (f : Nat → Trm), (((f 0 = t) ∧ (∀ n, (beta_red (f n) (f (Nat.succ n))))) → False)
+
+--the following is an inductive version of being strongly normalizable
+inductive SN : Trm → Prop
+  | sn : (∀ t', (beta_red t t') → SN t') → SN t
+
+--Both are logically equivalent
+lemma strongly_normalizable_iff_SN t :
+    strongly_normalizable t ↔ SN t := by
+  constructor
+  . contrapose
+    intro notsnt
+    have this : ∀ u , ¬ SN u → ∃ t', beta_red u t' ∧ ¬ SN t' := by
+      intro u notsnu
+      by_contra F
+      push_neg at F
+      apply notsnu (SN.sn F)
+    choose f w hw using this
+    let f' : Nat → {u // ¬ SN u} := fun n =>
+      Nat.iterate (fun (x : {u // ¬ SN u}) => ⟨f x.1 x.2, hw x.1 x.2⟩) n ⟨t, notsnt⟩
+    let f'' := (fun n => (f' n).1)
+    intro G
+    apply G f''
+    constructor
+    . rfl
+    . intro n
+      have rel := w (f' n).1 (f' n).2
+      have eq1 : ((f' n).1) = (f'' n) := by simp
+      have eq2 : (f (f' n).1 (f' n).2) = (f'' (Nat.succ n)) := by simp [Function.iterate_succ_apply']
+      simp [← eq1, ← eq2, rel]
+  . intro snt
+    induction snt
+    case sn t' _ ih =>
+      rintro f ⟨p , F⟩
+      let f' : ℕ → Trm := fun n => Nat.rec (f 1) (fun n _ => f (Nat.succ (Nat.succ n))) n
+      apply ih (f 1) (by rw [← p]; exact (F 0)) f'
+      constructor
+      . rfl
+      . intro n
+        induction n
+        case zero =>
+          exact (F 1)
+        case succ n _ =>
+          exact (F (Nat.succ (Nat.succ n)))
+
+--one-step reduction preserves being strongly normalizable
+lemma beta_red_preserves_SN (t : Trm) : SN t → ∀ t', beta_red t t' → SN t' := by
+  intro snt
+  cases snt
+  next F =>
+    exact F
+
+--multi-step reduction preserves being strongly normalizable
+lemma multi_red_preserves_SN (t t' : Trm) : SN t → multi_red t t' → SN t' := by
+  intro snt tmt'
+  induction tmt'
+  case mr_refl _ =>
+    exact snt
+  case mr_head t2 t3 _ t2bt3 ih =>
+    exact (beta_red_preserves_SN _ ih _ t2bt3)
+
+--for a locally closed term s, if applying s to t is strongly normalizing,
+--then t is strongly normalizing
+lemma SN_app1 t s : lc s → SN (t @ s) → SN t := by
+  intro lcs sn2ts
+  generalize h : (t @ s) = t' at sn2ts
+  induction sn2ts generalizing t with
+  | sn F IH =>
+    subst h
+    apply SN.sn
+    intro t' tbt'
+    apply IH (t' @ s) (beta_red.br_app1 t t' s lcs tbt') _ rfl
+
+-- If a term has two normal reducts, they must be the same
+lemma normal_is_unique (t : Trm) :
+    ∀ t1 t2, ((multi_red t t1) ∧ (normal t1)) ∧ ((multi_red t t2) ∧ (normal t2))
+    → t1 = t2 := by
+  intro t1 t2
+  rintro ⟨⟨tmt1, n1⟩ , ⟨tmt2, n2⟩⟩
+  have this : ∃ t3, multi_red t1 t3 ∧ multi_red t2 t3 := by
+    exact (beta_red_confluence t t1 t2 ⟨tmt1, tmt2⟩)
+  rcases this with ⟨t3, ⟨t1mt3, t2mt3⟩⟩
+  rw [normal_has_no_proper_multi_red t1 n1 t3 t1mt3]
+  rw [normal_has_no_proper_multi_red t2 n2 t3 t2mt3]
+
+-- Definition of strongly computable terms. The difference from Avigad's definition
+-- is that the definition is context free. This construction is also known as
+-- logical relations. The definition is valid for locally closed terms.
+@[simp]
+def SC : Typ → Set Trm
+  | typ_base => {t | (lc t) ∧ SN t}
+  | typ_arrow t1 t2 =>
+    {t | (lc t) ∧ (∀ u, ((lc u) ∧ (u ∈ SC t1)) → (t @ u) ∈ SC t2)}
+
+-- By definition, strongly computable terms are locally closed.
+lemma SC_regular A t : t ∈ (SC A) → lc t := by
+  intro H
+  induction A
+  case typ_base =>
+    exact H.1
+  case typ_arrow t1 t2 _ _ =>
+    exact H.1
+
+-- A term is neutral if it is not an abstraction.
+@[simp]
+def neutral : Trm → Prop
+| bvar _ => true
+| fvar _ => true
+| abs _ => false
+| app _ _ => true
+
+-- CR2 says that if t is strongly computable, then any multi-step reduct of t
+-- is also strongly computable.
+theorem CR2 : ∀ A t, (∀ t', t ∈ SC A → multi_red t t' → t' ∈ SC A) := by
+  intro A
+  induction A
+  case typ_base =>
+    intro t t' sct tmt'
+    exact ⟨(multi_red_regular _ _ tmt').2, (multi_red_preserves_SN _ _ sct.2 tmt')⟩
+  case typ_arrow A1 A2 _ ih2 =>
+    intro t t' sct tmt'
+    constructor
+    . apply (multi_red_regular _ _ tmt').2
+    . intro u H
+      have this1 : (t @ u) ∈ SC (A2) := (sct.2 u H)
+      apply ih2 (t @ u) (t' @ u) this1 (multi_red_app1 _ _ _ ⟨tmt', H.1⟩)
+
+-- CR1 says that strongly computable terms are strongly normalizing.
+-- CR3 says that if a locally closed term t is normal, also any
+-- one-step reduct of t is strongly computable, then t is strongly computable.
+theorem CR_1_3 : ∀ A t,
+    (t ∈ SC A → SN t) ∧ --CR1
+    (lc t → neutral t → (∀ t', beta_red t t' → t' ∈ SC A) → t ∈ SC A) := by --CR3
+  intro A
+  induction A
+  case typ_base =>
+    intro t
+    constructor
+    . exact (fun sct => sct.2) --CR1 base case
+    . exact (fun lct _ F => ⟨lct, SN.sn (fun s tbs => (F s tbs).2)⟩) --CR3 base case
+  case typ_arrow A1 A2 ih1 ih2 =>
+    intro t
+    constructor
+    . rintro ⟨_, H⟩ --CR1 arrow case
+      let ⟨x, p2⟩ := pick_fresh t ∅
+      simp at p2
+      have this2 : ($ x) ∈ SC A1 := by
+        apply (ih1 ($ x)).2 (lc_var x) (by simp)
+        intro t' nbt
+        cases nbt
+      have this3 : (app t ($ x)) ∈ SC A2 := H ($ x) ⟨lc_var x , this2⟩
+      have this4 : SN (app t ($ x)) := (ih2 (app t ($ x))).1 this3
+      apply (SN_app1 _ _ (lc_var x) this4)
+    . intro lct nt F --CR3 arrow case
+      constructor
+      . exact lct
+      . intro u Hu
+        have this1 : SN u := (ih1 _).1 Hu.2
+        induction this1
+        case sn u' _ ihu =>
+        apply (ih2 (t @ u')).2 (lc_app _ _ lct Hu.1) (by simp)
+        intro t' tubt'
+        cases tubt'
+        next a _ _ =>
+          simp [neutral] at nt
+        next a tba lcu =>
+          have this2 : a ∈ SC (A1 -> A2) := (F a tba)
+          apply (this2.2 u' Hu)
+        next c lct ubc =>
+          simp only
+          apply ihu c ubc
+          constructor
+          . apply (beta_red_regular _ _ ubc).2
+          . apply CR2 _ _ _ Hu.2 (beta_to_multi_red _ _ ubc)
+
+def CR1 A t := (CR_1_3 A t).1
+
+def CR3 A t := (CR_1_3 A t).2
+
+-- Free variables are always strongly computable.
+lemma SC_var A x : ($ x) ∈ SC A := by
+  induction A
+  case typ_base =>
+    constructor
+    . apply lc_var x
+    . apply SN.sn
+      intro t tbx
+      cases tbx
+  case typ_arrow A1 A2 _ _ =>
+    apply CR3 _ _ (lc_var x) (by simp)
+    intro t' bred
+    cases bred
+
+lemma SC_lambda_lemma A1 A2 t : lc (λ t)
+    → (∀ u x, x ∉ fv t → u ∈ SC A1 → ([x // u] (open₀ t ($ x))) ∈ SC A2)
+    → ∃ y, (open₀ t ($ y)) ∈ SC A2 := by
+  intro _ F
+  let ⟨y, hy⟩ := pick_fresh t ∅
+  simp at hy
+  have this : ($ y) ∈ SC A1 := SC_var A1 y
+  have this2 : (open₀ t ($ y)) ∈ SC A2 := by
+    rw [subst_intro t ($ y) (lc_var y) y hy]
+    exact (F ($ y) y hy this)
+  exact ⟨y, this2⟩
+
+-- Criteria for strongly computable lambda terms:
+-- Suppose for all variable x not occured in t and strongly computable u, we have
+-- [x//u]tˣ is strongly computable. Then λt is strongly computable.
+theorem SC_lambda A1 A2 t : lc (λ t)
+    → (∀ u x, x ∉ fv t → u ∈ SC A1 → ([x // u] (open₀ t ($ x))) ∈ SC A2)
+    → (λ t) ∈ SC (A1 -> A2) := by
+  intro lct F
+  have this := (SC_lambda_lemma _ _ _ lct F)
+  rcases this with ⟨y, hy⟩
+  constructor
+  . exact lct
+  . intro u Hu
+    have snu := CR1 _ _ Hu.2
+    have snt := CR1 _ _ hy
+    generalize h : (open₀ t ($ y)) = t' at snt
+    induction snt generalizing t with
+    | sn _ iht' =>
+      rw [← h] at iht'
+      induction snu
+      case sn u' _ ihu' =>
+        apply CR3 _ _ (lc_app _ _ lct Hu.1) (by simp)
+        intro t'' bred
+        cases bred
+        next lct' lcu' =>
+          let ⟨z, hz⟩ := pick_fresh t {0}
+          simp at hz
+          push_neg at hz
+          rw [subst_intro _ _ Hu.1 z hz.2]
+          apply (F u' z hz.2 Hu.2)
+        next t1' t'bt1' lcu' =>
+          cases t'bt1'
+          next t'' L a =>
+            let ⟨x, hx⟩ := pick_fresh t (L ∪ (fv t''))
+            simp at hx
+            push_neg at hx
+            have this3 : beta_red (open₀ t ($ y))  (open₀ t'' ($ y)) := by
+              rw [subst_intro t ($ y) (lc_var y) x hx.2.2]
+              rw [subst_intro t'' ($ y) (lc_var y) x hx.2.1]
+              apply beta_rename _ _ _ _ (a x hx.1)
+            apply (iht' (open₀ t'' ($ y)) this3 t''
+                (beta_red_regular _ _ (beta_red.br_abs _ _ _ a)).2)
+            intro u z hz scu
+            rw [← subst_intro t'' u (SC_regular _ _ scu) z hz]
+            have this4 : open₀ t u ∈ SC A2 := by
+              rw [subst_intro t u (SC_regular _ _ scu) x hx.2.2]
+              apply F u x hx.2.2 scu
+            apply CR2 _ _ _ this4
+            apply beta_to_multi_red
+            rw [subst_intro t'' u (SC_regular _ _ scu) x hx.2.1]
+            rw [subst_intro t u (SC_regular _ _ scu) x hx.2.2]
+            apply beta_red_subst_out _ _ _ _ ⟨a x hx.1, (SC_regular _ _ scu)⟩
+            apply CR2 _ _ _ hy (beta_to_multi_red _ _ this3)
+            rfl
+        next u1' lct' u'bu1 =>
+          apply ihu' u1' u'bu1
+          have this5 := (beta_red_regular _ _ u'bu1).2
+          exact ⟨this5, CR2 _ _ _ Hu.2 (beta_to_multi_red _ _ u'bu1)⟩
+          intro t1 bred t2 typ2 F2 op2 q2
+          apply CR2
+          apply iht' t1 bred _ typ2 F2 op2 q2
+          apply (beta_to_multi_red _ _ (beta_red.br_app2 _ _ _ (typ2) u'bu1))
+
+-- We can generalize the previous theorem:
+-- Suppose for all strongly computable u, the opened term tᵘ is strongly computable.
+-- Then λt is strongly computable.
+theorem SC_lambda_open A1 A2 t : lc (λ t)
+    → (∀ u, u ∈ SC A1 → (open₀ t u) ∈ SC A2)
+    → (λ t) ∈ SC (A1 -> A2) := by
+  intro typt F
+  apply SC_lambda _ _ _ typt
+  intro u x fvx scu
+  rw [← subst_intro _ _ (SC_regular _ _ scu) x fvx]
+  apply F u scu
+
+-- Fundamental lemma about logical relations:
+-- Suppose (x1:A1, x2:A2, ..., xn:An) ⊢ t : A. Then for any strongly computable ui:Ai,
+-- we have ([x1//u1, x2//u2, ..., xn//un] t) is strongly computable.
+lemma SC_subst t A : typing Γ t A
+    → (f : (context_terms Γ) → Trm)
+    → (∀ x (h : x ∈ (context_terms Γ)), (f ⟨x, h⟩) ∈ SC (context_type Γ ⟨x, h⟩))
+    → (multi_subst (context_terms Γ) f t) ∈ SC A := by
+  intro typt
+  induction typt
+  case typ_var Δ y T vld bnd =>
+    intro f Hf
+    simp only [multi_subst]
+    by_cases h : y ∈ context_terms Δ
+    . simp [h, ← context_type_eq_bind Δ ⟨y, h⟩ T vld bnd]
+      apply (Hf y h)
+    . simp [h]
+      apply SC_var
+  case typ_abs L Δ u T1 T2 a ih =>
+    intro f Hf
+    apply SC_lambda_open
+    rw [← multi_subst]
+    apply multi_subst_lc _ _ (typing_regular _ _ _ (typ_abs L Δ u T1 T2 a))
+    exact (fun x hx => (SC_regular _ _ (Hf x hx)))
+    intros u1 scu1
+    let ⟨x, hx⟩ := pick_fresh u L
+    simp at hx
+    push_neg at hx
+    have this : (∀ y (s : y ∈ (context_terms ((x, T1) :: Δ))),
+        ((add_term Δ f u1 x T1) ⟨y, s⟩) ∈ SC (context_type ((x, T1) :: Δ) ⟨y, s⟩)) := by
+      intro y s
+      by_cases p : y = x
+      . simp [p, scu1]
+      . simp [p] at s ⊢
+        apply Hf y s
+    have this2 := ih x hx.1 (add_term Δ f u1 x T1) this
+    rw [multi_subst_open_lemma_2] at this2
+    exact this2
+    apply (SC_regular _ _ scu1)
+    apply hx.2
+    exact (fun y s => (SC_regular _ _ (Hf y s)))
+  case typ_app Δ t1 t2 T1 T2 _ typt2 ih1 ih2 =>
+    intro f Hf
+    cases (ih1 f Hf)
+    next L R =>
+      apply R (multi_subst (context_terms Δ) f t2)
+      constructor
+      . apply multi_subst_lc
+        apply (typing_regular _ _ _ typt2)
+        exact (fun x hx => (SC_regular _ _ (Hf x hx)))
+      . apply (ih2 f Hf)
+
+-- Final theorem:
+-- By CR1 and substitution lemma, we have every typeable term is strongly normalizing.
+theorem beta_red_strongly_normalizing t T : typing [] t T → SN t := by
+  intro typt
+  apply CR1 T t
+  let ⟨x, hx⟩ := pick_fresh t ∅
+  simp at hx
+  let f : context_terms [(x, T)] → Trm := fun _ => ($ x)
+  have this : multi_subst (context_terms [(x, T)]) f t = t := by
+    rw [multi_subst_at_singleton]
+    rw [subst_fresh _ _ _ hx]
+  rw [← this]
+  apply SC_subst
+  apply typing_weakening [] [(x, T)] _ _ typt
+  apply valid_push _ _ _ (valid_ctx.valid_nil) (by simp)
+  exact (fun y hy => SC_var _ _)
