Stlc/typing.lean
@@ -1,17 +1,16 @@
 import Stlc.basics
 import Stlc.open_close
 import Stlc.context
-import Mathlib.Data.Finset.Basic
-import Mathlib.Data.List.Basic
+import Stlc.reductions
 
 open Typ
 open Trm
-open List 
+open List
 
 --Typing judgment
 inductive typing : context → Trm → Typ → Prop
 | typ_var (Γ : context) (x : ℕ) (T : Typ) : (valid_ctx Γ) → (binds x T Γ) → (typing Γ ($ x) T)
-| typ_abs (L : Finset ℕ) (Γ : context) (t : Trm) (T1 T2 : Typ) : 
+| typ_abs (L : Finset ℕ) (Γ : context) (t : Trm) (T1 T2 : Typ) :
         ((x : ℕ) → x ∉ L → (typing ((x, T1) :: Γ) (open₀ t ($ x)) T2)) → (typing Γ (abs t) (typ_arrow T1 T2))
 | typ_app (Γ : context) (t₁ t₂ : Trm) (T1 T2 : Typ) :
         (typing Γ t₁ (typ_arrow T1 T2)) → (typing Γ t₂ T1) → typing Γ (app t₁ t₂) T2
@@ -27,11 +26,10 @@ lemma typing_valid_ctx  Γ e T : typing Γ e T → valid_ctx Γ := by
   case typ_var _ _ _ h _ =>
     exact h
   case typ_abs L φ t T1 _ _ f =>
-    have p := pick_fresh t L
-    rcases p with ⟨p1, p2⟩ 
+    let ⟨p1, p2⟩ := pick_fresh t L
     simp at p2
     push_neg at p2
-    apply valid_remove_cons 
+    apply valid_remove_cons
     apply (f p1 p2.1)
   case typ_app _ _ _ _ _ _ _ h1 _ =>
     exact h1
@@ -39,21 +37,20 @@ lemma typing_valid_ctx  Γ e T : typing Γ e T → valid_ctx Γ := by
 
 --Weakining Rule
 lemma typing_weakening_strengthened' (Γ Δ Ψ' : context) (t : Trm) (T : Typ) :
-    typing Ψ' t T → 
-    (Ψ : context) → Ψ' = Ψ ++ Γ → 
-    valid_ctx (Ψ ++ Δ ++ Γ) ->
-    typing (Ψ ++ Δ ++ Γ) t T := by
+    typing Ψ' t T → (Ψ : context) → Ψ' = Ψ ++ Γ
+    → valid_ctx (Ψ ++ Δ ++ Γ)
+    → typing (Ψ ++ Δ ++ Γ) t T := by
   intro H
   induction H
   case typ_var φ x T' _ fT' =>
     intro φ p f
     apply typ_var
     exact f
-    rw [p] at fT' 
+    rw [p] at fT'
     exact (binds_weaken _ _ _ _ _ fT' f)
   case typ_abs L φ' s T1 T2 _ fT2 =>
     intro φ p f
-    apply typ_abs (L ∪ dom (φ ++ Δ ++ Γ))
+    apply typ_abs (L ∪ context_terms (φ ++ Δ ++ Γ))
     intro x hx
     simp at hx
     push_neg at hx
@@ -63,17 +60,17 @@ lemma typing_weakening_strengthened' (Γ Δ Ψ' : context) (t : Trm) (T : Typ) :
     exact f
     simp [append_cons]
     intro q
-    exact (hx.2 ((dom_iff_in_list x _).mpr q))
+    exact (hx.2 ((context_terms_iff_in_list x _).mpr q))
   case typ_app φ' t1 t2 T1 T2 _ _ fT1 fT2 =>
-    intro φ p f 
+    intro φ p f
     apply typ_app
     exact (fT1 φ p f)
-    exact (fT2 φ p f)    
-    
+    exact (fT2 φ p f)
+
 lemma typing_weakening_strengthened (Γ Δ Ψ : context) (t : Trm) (T : Typ) :
-    typing (Ψ ++ Γ) t T ->
-    valid_ctx (Ψ ++ Δ ++ Γ) ->
-    typing (Ψ ++ Δ ++ Γ) t T := by
+    typing (Ψ ++ Γ) t T
+    → valid_ctx (Ψ ++ Δ ++ Γ)
+    → typing (Ψ ++ Δ ++ Γ) t T := by
   intro H p
   apply (typing_weakening_strengthened' _ _ (Ψ ++ Γ))
   exact H
@@ -81,9 +78,8 @@ lemma typing_weakening_strengthened (Γ Δ Ψ : context) (t : Trm) (T : Typ) :
   exact p
 
 lemma typing_weakening (Γ Δ : context) (t : Trm) (T : Typ) :
-    typing (Γ) t T ->
-    valid_ctx (Δ ++ Γ) ->
-    typing (Δ ++ Γ) t T := by
+    typing (Γ) t T → valid_ctx (Δ ++ Γ)
+    → typing (Δ ++ Γ) t T := by
   intro H p
   rw [← nil_append (Δ ++ Γ)] at p
   apply (typing_weakening_strengthened Γ Δ [])
@@ -91,12 +87,21 @@ lemma typing_weakening (Γ Δ : context) (t : Trm) (T : Typ) :
   exact H
   exact p
 
+lemma typing_weakening_head (Γ : context) (t : Trm) (T S : Typ) (x : ℕ):
+    ¬ (in_context x Γ) → typing Γ t T
+    → typing ((x , S) :: Γ) t T := by
+  intro notxl typt
+  rw [← nil_append ((x , S) :: Γ), append_cons, nil_append]
+  apply typing_weakening _ _ _ _ typt
+  apply valid_push
+  apply (typing_valid_ctx _ _ _ typt)
+  exact notxl
+
 --Substitution Rule
 lemma typing_subst_var_case Γ Δ u S T z x :
-    binds x T (Δ ++ (z, S) :: Γ) → 
-    valid_ctx (Δ ++ (z, S) :: Γ) → 
-    typing Γ u S → 
-    typing (Δ ++ Γ) ([z // u] ($ x)) T := by
+    binds x T (Δ ++ (z, S) :: Γ)
+    → valid_ctx (Δ ++ (z, S) :: Γ)
+    → typing Γ u S → typing (Δ ++ Γ) ([z // u] ($ x)) T := by
   intro b v t
   simp only [subst]
   by_cases hxz : x = z
@@ -119,14 +124,15 @@ lemma typing_subst_var_case Γ Δ u S T z x :
     push_neg at hxz
     exact hxz
 
-lemma typing_regular (t : Trm) (T : Typ) (Γ : context) : typing Γ t T -> lc t := by
+lemma typing_regular (t : Trm) (T : Typ) (Γ : context) :
+    typing Γ t T -> lc t := by
   intro H
   induction H
   case typ_var _ x _ _ _ =>
     exact (lc.lc_var x)
   case typ_abs L _ u _ _ _ h' =>
     apply (lc.lc_abs u L)
-    intro x hx 
+    intro x hx
     exact (h' x hx)
   case typ_app _ t1 t2 _ _ _ _ f1 f2 =>
     apply (lc.lc_app)
@@ -134,11 +140,9 @@ lemma typing_regular (t : Trm) (T : Typ) (Γ : context) : typing Γ t T -> lc t 
     exact f2
 
 lemma typing_subst_strengthened' Γ Δ' t u S T z :
-    typing Δ' t T →
-    ((φ : context) → Δ' = (φ ++ (z, S) :: Γ) → 
-    typing (φ ++ (z, S) :: Γ) t T ->
-    typing Γ u S ->
-    typing (φ ++ Γ) ([z // u] t) T ) := by
+    typing Δ' t T → ((φ : context) → Δ' = (φ ++ (z, S) :: Γ)
+    → typing (φ ++ (z, S) :: Γ) t T
+    → typing Γ u S → typing (φ ++ Γ) ([z // u] t) T ) := by
   intro H
   induction H
   case typ_var ψ x X h h' =>
@@ -148,11 +152,11 @@ lemma typing_subst_strengthened' Γ Δ' t u S T z :
     exact h'
     rw [p] at h
     exact h
-    exact f 
+    exact f
   case typ_abs L ψ s S1 S2 h h' =>
     intro Δ p _ f
     simp only [subst]
-    apply typ_abs (L ∪ dom (Δ ++ Γ) ∪ {z}) (Δ ++ Γ) ([z // u] s) S1 S2
+    apply typ_abs (L ∪ context_terms (Δ ++ Γ) ∪ {z}) (Δ ++ Γ) ([z // u] s) S1 S2
     intro x hx
     rw [subst_open_var s u]
     simp at hx
@@ -179,8 +183,8 @@ lemma typing_subst_strengthened' Γ Δ' t u S T z :
     exact f
 
 lemma typing_subst_strengthened Γ Δ t u S T z :
-    typing (Δ ++ (z, S) :: Γ) t T ->
-    typing Γ u S ->
+    typing (Δ ++ (z, S) :: Γ) t T →
+    typing Γ u S →
     typing (Δ ++ Γ) ([z // u] t) T := by
   intro H p
   apply (typing_subst_strengthened')
@@ -188,11 +192,11 @@ lemma typing_subst_strengthened Γ Δ t u S T z :
   rfl
   exact H
   exact p
-  
+
 lemma typing_subst Γ t u S T z :
-    typing ((z, S) :: Γ) t T ->
-    typing Γ u S ->
-    typing Γ ([z // u] t) T := by 
+    typing ((z, S) :: Γ) t T →
+    typing Γ u S →
+    typing Γ ([z // u] t) T := by
   intro H p
   rw [← nil_append ((z, S) :: Γ)] at H
   rw [← nil_append Γ]
@@ -202,13 +206,13 @@ lemma typing_subst Γ t u S T z :
 --------------------------------------------
 
 lemma typing_rename Γ x y t T1 T2 :
-    x ∉ fv t →  ¬ (in_list x Γ) →
-    y ∉ fv t →  ¬ (in_list y Γ) →
-    typing ((x, T1) :: Γ) (open₀ t ($ x)) T2 →
-    typing ((y, T1) :: Γ) (open₀ t ($ y)) T2 := by
-  intro hx fx _ fy R 
+    x ∉ fv t →  ¬ (in_context x Γ)
+    → y ∉ fv t →  ¬ (in_context y Γ)
+    → typing ((x, T1) :: Γ) (open₀ t ($ x)) T2
+    → typing ((y, T1) :: Γ) (open₀ t ($ y)) T2 := by
+  intro hx fx _ fy R
   by_cases hxy : x = y
-  . rwa [hxy] at R 
+  . rwa [hxy] at R
   . have ok_ctx : valid_ctx Γ := by
       apply valid_remove_cons
       apply typing_valid_ctx
@@ -230,17 +234,69 @@ lemma typing_rename Γ x y t T1 T2 :
     simp
 
 lemma typing_abs_intro Γ x t T1 T2 :
-    x ∉ fv t →  ¬ (in_list x Γ) → 
-    typing ((x, T1) :: Γ) (open₀ t ($ x)) T2 → 
-    typing Γ (abs t) (T1 -> T2) := by
+    x ∉ fv t →  ¬ (in_context x Γ)
+    → typing ((x, T1) :: Γ) (open₀ t ($ x)) T2
+    → typing Γ (abs t) (T1 -> T2) := by
   intro hx fx R
-  apply typ_abs (fv t ∪ dom Γ)
+  apply typ_abs (fv t ∪ context_terms Γ)
   intro y hy
   simp at hy
   push_neg at hy
   apply (typing_rename _ _ _ _ _ _ hx fx)
   exact hy.1
-  exact (fun q => hy.2 ((dom_iff_in_list _ _).mpr q))
+  exact (fun q => hy.2 ((context_terms_iff_in_list _ _).mpr q))
   exact R
 
+lemma preservation_beta_red E e T :
+    typing E e T
+    → ((e' : Trm) →  beta_red e e' → typing E e' T) := by
+  intro H
+  induction H
+  case typ_var φ x S _ _ =>
+    intro e' p
+    cases p
+  case typ_abs L φ t S1 S2 _ a_ih =>
+    intro e' p
+    cases p
+    next t1' L' a' =>
+      simp only
+      apply typ_abs (L' ∪ L)
+      intro x hx
+      simp at hx
+      push_neg at hx
+      apply (a_ih x hx.2 (open₀ t1' ($ x)))
+      apply (a' x hx.1)
+  case typ_app φ t1 t2 S1 S2 f1 f2 h1 h2 =>
+    intro e' p
+    cases p
+    next e1 lce1 g =>
+      cases f1
+      next L h =>
+        simp only
+        let ⟨x, hx⟩ := pick_fresh e1 L
+        have q : lc t2 := by
+          apply (typing_regular _ _ _ f2)
+        simp at hx
+        push_neg at hx
+        rw [subst_intro e1 t2 q x hx.2]
+        apply (typing_subst)
+        exact (h x hx.1)
+        exact f2
+    next e1 eve1 lct2 =>
+      apply typ_app
+      apply (h1 e1 eve1)
+      exact f2
+    next e2 lct1 eve2 =>
+      apply typ_app
+      exact f1
+      apply (h2 e2 eve2)
 
+lemma preservation_multi_red E e T :
+    typing E e T
+    → ((e' : Trm) →  multi_red e e' → typing E e' T) := by
+  intro H e' eme'
+  induction eme'
+  next _ =>
+    exact H
+  next t2 t3 _ t2bt3 ih =>
+      apply (preservation_beta_red _ _ _ ih _ t2bt3)
